updated examples + Load

src/Dafny/examples/simple.i.dfy
@@ -1,9 +1,12 @@
 include "../llvm.i.dfy"
 include "../control_flow.i.dfy"
+include "generalInstructions.i.dfy"
+
 
 module simple_functions {
     import opened LLVM_def
     import opened control_flow
+    import opened general_instructions
 
 
 function method{:opaque} lvm_code_Empty_Test():lvm_code
@@ -50,88 +53,6 @@ lemma lvm_lemma_Empty_Test(lvm_b0:lvm_codes, lvm_s0:lvm_state, lvm_sN:lvm_state,
     lvm_sM := lvm_lemma_empty(lvm_s0, lvm_sM);
 }
 
-function method{:opaque}lvm_code_Add(dst:lvm_operand_opr, size:nat, src1:lvm_operand_opr,src2:lvm_operand_opr):lvm_code
-   requires src1.D?
-   requires src1.d.Int?
-   requires src2.D?
-   requires src2.d.Int?
-    requires typesMatch(src1.d,src2.d)
-
-{
-   Ins(ADD(dst, size,src1,src2))
-}
-lemma lvm_lemma_Add(lvm_b0:lvm_codes, lvm_s0:lvm_state, lvm_sN:lvm_state, 
-            dst:lvm_operand_opr, size:nat, src1:lvm_operand_opr,src2:lvm_operand_opr,o:operand)
-  returns (lvm_bM:lvm_codes, lvm_sM:lvm_state)
-  requires src1.D?
-  requires src1.d.Int?
-  requires src2.D?
-  requires src2.d.Int?
-  requires typesMatch(src1.d,src2.d)
-  requires lvm_require(lvm_b0, lvm_code_Add(dst, size,src1,src2), lvm_s0, lvm_sN,dst)
-  requires lvm_is_dst_opr(dst, lvm_s0)
-  requires lvm_is_src_opr(src1, lvm_s0)
-  requires lvm_get_ok(lvm_s0)
-
-  requires ValidOperand(lvm_s0,src1);
-  requires OperandContents(lvm_s0,src1).Int?;
-  requires ValidOperand(lvm_s0,src2);
-  requires OperandContents(lvm_s0,src2).Int?;
-  requires ValidOperand(lvm_s0,dst);
-  requires OperandContents(lvm_s0,dst).Int?;
-
-  requires ValidOperand(lvm_s0,dst);
-  requires typesMatch(OperandContents(lvm_s0,src1),OperandContents(lvm_s0,src2))
-  requires OperandContents(lvm_s0,src2).Int?;
-  requires lvm_code_Add(dst, size,src1,src2).Ins?;
-  requires ValidOperand(lvm_s0,dst)
-// //   
-  ensures  lvm_ensure(lvm_b0, lvm_bM, lvm_s0, lvm_sM, lvm_sN,dst)
-  ensures  lvm_get_ok(lvm_sM)
-  ensures  ValidOperand(lvm_sM,dst)
-  ensures  ValidOperand(lvm_sM,src1)
-  ensures OperandContents(lvm_sM,src1).Int?;
-  ensures  ValidOperand(lvm_sM,src2)
-  ensures OperandContents(lvm_sM,src2).Int?;
-  ensures typesMatch(OperandContents(lvm_sM,src1),OperandContents(lvm_sM,src2))
-
-  ensures  OperandContents(lvm_sM,dst).Int?;
-  ensures  lvm_state_eq(lvm_sM, lvm_update_mem( lvm_sM, lvm_update_all(lvm_sM, lvm_s0)))
-  ensures  lvm_state_eq(lvm_sM, lvm_update_ok(lvm_sM, lvm_update_all( lvm_sM, lvm_s0)))
-  ensures  forall s2 :: evalCode(lvm_b0.hd, lvm_s0, s2,o) ==> s2.ok
-  ensures OperandContents(lvm_sM, dst).val == evalADD(OperandContents(lvm_s0,dst).itype.size,OperandContents(lvm_s0,src1),OperandContents(lvm_s0,src2)).val;
-  ensures ToTwosComp(OperandContents(lvm_sM, dst)).val == 
-          (OperandContents(lvm_s0, src1).val + OperandContents(lvm_s0, src2).val) % Pow256(OperandContents(lvm_s0, src1).itype.size)
-
-{
-    reveal_lvm_code_Add();
-    reveal_evalCodeOpaque();
-    reveal_eval_code();
-    assert lvm_code_Add(dst, size,src1,src2).Ins?;
-    var addIns := lvm_code_Add(dst, size,src1,src2).ins;
-    assert ValidInstruction(lvm_s0,addIns);
-
-    assert  ValidRegOperand(lvm_s0, dst);
-    assert ValidState(lvm_s0);
-    var lvm_old_s:lvm_state := lvm_s0;
-    assert evalCode_lax(lvm_Block(lvm_b0), lvm_s0, lvm_sN,dst);
-    assert lvm_s0.ok;
-    assert eval_code(lvm_Block(lvm_b0), lvm_s0, lvm_sN,dst);
-
-    ghost var lvm_ltmp1, lvm_cM:lvm_code, lvm_ltmp2 := lvm_lemma_block(lvm_b0, lvm_s0, lvm_sN,dst);
-    lvm_sM := lvm_ltmp1;
-    lvm_bM := lvm_ltmp2;
-    assert lvm_b0.tl == lvm_bM;
-    assert ValidState(lvm_s0);
-    assert lvm_s0.ok;
-    assert ValidState(lvm_sM);
-    assert ValidOperand(lvm_sM,dst);
-    assert evalIns(lvm_code_Add(dst, size,src1,src2).ins,lvm_s0,lvm_sM,dst);
-    assert evalUpdate(lvm_s0, dst, evalADD(OperandContents(lvm_s0,dst).itype.size,OperandContents(lvm_s0,src1),OperandContents(lvm_s0,src2)),lvm_sM);
-    assert  ValidData(lvm_sM,evalADD(OperandContents(lvm_s0,dst).itype.size,OperandContents(lvm_s0,src1),OperandContents(lvm_s0,src2)));
-    assert OperandContents(lvm_sM, dst).val == evalADD(OperandContents(lvm_s0,dst).itype.size,OperandContents(lvm_s0,src1),OperandContents(lvm_s0,src2)).val;
-    reveal_evalCodeOpaque();
-}
 
 ////
     // test(src){
@@ -212,8 +133,9 @@ function method {:opaque} lvm_code_Add_Multiple(dst:lvm_operand_opr, size:nat, s
       var val2 := D(Int(5,src1.d.itype));
       assert val.d.Int?;
 
-      lvm_Block(lvm_CCons(Ins(ADD(dst,size,src1,val)),
-                lvm_CCons(Ins(ADD(dst,size,src1,val2)),lvm_CNil())))
+          lvm_Block(lvm_CCons(Ins(ADD(dst,size,src1,val)),
+                lvm_CCons(Ins(ADD(dst,size,src1,val2)),
+                lvm_CCons(Ins(RET(void)),lvm_CNil()))))
 
 }
 
@@ -250,6 +172,8 @@ lemma lvm_lemma_Add_Multiple(lvm_b0:lvm_codes, lvm_s0:lvm_state, lvm_sN:lvm_stat
     reveal_eval_code();
     reveal_evalCodeOpaque();
     reveal_lvm_code_Add();
+    reveal_lvm_RET();
+
     assert lvm_code_Add_Multiple(dst, size,src1).block.hd.Ins?;
 
     assert ValidState(lvm_s0);
@@ -270,6 +194,13 @@ lemma lvm_lemma_Add_Multiple(lvm_b0:lvm_codes, lvm_s0:lvm_state, lvm_sN:lvm_stat
     assert evalCode_lax(lvm_Block(lvm_b1), lvm_s0, lvm_sM,dst);
     assert OperandContents(lvm_s0,dst).Int?;
 
+    // assert evalUpdate(lvm_s0, dst, evalADD(size,OperandContents(lvm_s0,src1),OperandContents(lvm_s0,val)),lvm_sM);
+    assert evalCode(lvm_Block(lvm_b1), lvm_s0, lvm_sM,dst);
+    assert evalBlock(lvm_Block(lvm_b1).block, lvm_s0, lvm_sM,dst);
+    assert lvm_Block(lvm_b1).block.hd == Ins(ADD(dst, size,src1,val));
+    assert  exists r' ::  evalCode(lvm_b1.hd, lvm_s0, r',dst);
+    assert  exists r' ::  evalIns(lvm_b1.hd.ins, lvm_s0, r',dst);
+
     var val2 := D(Int(5,src1.d.itype));
     var step1 := evalADD(OperandContents(lvm_s0,dst).itype.size,OperandContents(lvm_s0,src1),val.d);
 
@@ -288,8 +219,14 @@ lemma lvm_lemma_Add_Multiple(lvm_b0:lvm_codes, lvm_s0:lvm_state, lvm_sN:lvm_stat
         == evalADD(OperandContents(lvm_s2,dst).itype.size,OperandContents(lvm_s2,src1),val2.d).val;
   
     assert OperandContents(lvm_s3, dst).val  == step2.val;
-    assert lvm_b3.CNil?;
-    lvm_sM := lvm_lemma_empty(lvm_s3,lvm_sM);
+    // assert lvm_b3.CNil?;
+    assert lvm_b3.hd.ins == RET(D(Void));
+
+    
+    ghost var lvm_b4, lvm_s4 := lvm_lemma_Ret(lvm_b3, lvm_s3, lvm_sM, dst, D(Void));
+    assert lvm_b4.CNil?;
+
+    lvm_sM := lvm_lemma_empty(lvm_s4,lvm_sM);
     assert   OperandContents(lvm_sM, dst).val  == step2.val;
 
     assert evalCode_lax(lvm_cM, lvm_s0, lvm_sM,dst);
@@ -302,6 +239,151 @@ lemma lvm_lemma_Add_Multiple(lvm_b0:lvm_codes, lvm_s0:lvm_state, lvm_sN:lvm_stat
     reveal_evalCodeOpaque();
 }
 
+
+
+////
+
+function method {:opaque} lvm_code_Add_Multiple1(dst:lvm_operand_opr, size:nat, src1:lvm_operand_opr, src2:lvm_operand_opr): (out:lvm_code)
+    requires src1.D?;
+    requires src1.d.Int?;
+    requires src2.D?;
+    requires src2.d.Int?;
+    ensures out.Block?;
+    ensures out.block.lvm_CCons?;
+    ensures out.block.hd.Ins?;
+
+{
+      reveal_IntFits();
+      var val := D(Int(4,src1.d.itype));
+      assert val.d.Int?;
+      var void := D(Void);
+
+      var val2 := D(Int(5,src2.d.itype));
+      assert val.d.Int?;
+
+      // var void := D(Void);
+
+      lvm_Block(lvm_CCons(Ins(ADD(src2,size,src1,val)),
+                lvm_CCons(Ins(ADD(dst,size,src2,val2)),
+                lvm_CCons(Ins(RET(void)),lvm_CNil()))))
+
+}
+
+lemma lvm_lemma_Add_Multiple1(lvm_b0:lvm_codes, lvm_s0:lvm_state, lvm_sN:lvm_state, 
+            dst:lvm_operand_opr, size:nat, src1:lvm_operand_opr,src2:lvm_operand_opr,o:operand)
+  returns (lvm_bM:lvm_codes, lvm_sM:lvm_state)
+  requires src1.D?;
+  requires src1.d.Int?;
+  requires src2.D?;
+  requires src2.d.Int?;
+  requires lvm_require(lvm_b0, lvm_code_Add_Multiple1(dst, size,src1,src2), lvm_s0, lvm_sN,dst)
+  requires lvm_is_dst_opr(dst, lvm_s0)
+  requires lvm_is_dst_opr(src2, lvm_s0)
+  requires lvm_is_src_opr(src1, lvm_s0)
+  requires lvm_get_ok(lvm_s0)
+
+  requires ValidOperand(lvm_s0,src1);
+  requires OperandContents(lvm_s0,src1).Int?;
+  requires ValidOperand(lvm_s0,src2);
+  requires OperandContents(lvm_s0,src2).Int?;
+  requires ValidOperand(lvm_s0,dst);
+  requires OperandContents(lvm_s0,dst).Int?;
+//   
+  ensures  lvm_ensure(lvm_b0, lvm_bM, lvm_s0, lvm_sM, lvm_sN,dst)
+  ensures  lvm_get_ok(lvm_sM) 
+  ensures ValidOperand(lvm_sM,dst)
+  ensures OperandContents(lvm_sM,dst).Int?;
+  ensures OperandContents(lvm_s0,dst).Int?;
+
+  // ensures  OperandContents(lvm_sM, dst).val == evalADD(OperandContents(lvm_s0,dst).itype.size,OperandContents(lvm_s0,src1),D(Int(5,src1.d.itype)).d).val;
+  ensures ToTwosComp(OperandContents(lvm_sM, dst)).val == 
+          (OperandContents(lvm_s0, src1).val + D(Int(5,src1.d.itype)).d.val + D(Int(4,src1.d.itype)).d.val ) % Pow256(OperandContents(lvm_s0, src1).itype.size)
+  ensures  lvm_state_eq(lvm_sM, lvm_update_ok(lvm_sM, lvm_update_all( lvm_sM, lvm_s0)))
+{
+    reveal_lvm_code_Add_Multiple1();
+    reveal_eval_code();
+    reveal_evalCodeOpaque();
+    reveal_lvm_code_Add();
+      reveal_lvm_RET();
+
+    assert lvm_code_Add_Multiple1(dst, size,src1,src2).block.hd.Ins?;
+
+    assert ValidState(lvm_s0);
+    var lvm_old_s:lvm_state := lvm_s0;
+    assert evalCode(lvm_Block(lvm_b0), lvm_s0, lvm_sN,dst);
+    assert eval_code(lvm_Block(lvm_b0), lvm_s0, lvm_sN,dst);
+
+    ghost var lvm_ltmp1, lvm_cM:lvm_code, lvm_ltmp2 := lvm_lemma_block(lvm_b0, lvm_s0, lvm_sN,dst);
+    lvm_sM := lvm_ltmp1;
+    lvm_bM := lvm_ltmp2;
+    var lvm_b1:lvm_codes := lvm_get_block(lvm_cM);
+    assert lvm_b1.lvm_CCons?;
+    reveal_IntFits();
+    var val := D(Int(4,src1.d.itype));
+    assert val.d.Int?;
+    assert lvm_b1.hd == lvm_code_Add(src2, size,src1,val);
+    assert ValidState(lvm_s0);
+    // src2 := evalADD(size,OperandContents(lvm_s0,src1),OperandContents(lvm_s0,val));
+    assert lvm_code_Add(src2, size,src1,val).ins == (ADD(src2, size,src1,val));
+    assert ValidInstruction(lvm_s0,(ADD(src2, size,src1,val)));
+    assert ValidData(lvm_sM,evalADD(size,OperandContents(lvm_s0,src1),OperandContents(lvm_s0,val)));
+    // assert src2.D?;
+    // assert src2.d == evalADD(size,OperandContents(lvm_s0,src1),OperandContents(lvm_s0,val));
+    // assert lvm_s0 == lvm_sM;
+      //  assert evalCode_lax(lvm_Block(lvm_b1), lvm_s0, lvm_sM,src2);
+      assert lvm_b1.hd.Ins?;
+      assert lvm_b1.hd.ins.dst == src2;
+      assert lvm_Block(lvm_b1).block.hd == Ins(ADD(src2, size,src1,val));
+      // assert  exists r' ::  evalCode(lvm_b1.hd, lvm_s0, r',src2);
+        assert evalCode(lvm_Block(lvm_b1), lvm_s0, lvm_sM,dst);
+
+    // assert  exists r' ::  evalIns(lvm_b1.hd.ins, lvm_s0, r',src2);
+      // assert  evalIns(lvm_b1.hd.ins, lvm_s0, lvm_sM,dst);
+
+      // assert exists r' :: evalCode(lvm_b1.hd, lvm_s0, r',dst);
+
+      assert evalBlock(lvm_b1,lvm_s0, lvm_sM,dst);
+      assert evalCode(lvm_Block(lvm_b1), lvm_s0, lvm_sM,dst);
+      assert  exists r' ::  evalIns(lvm_b1.hd.ins, lvm_s0, r',dst); // ???  
+
+    var val2 := D(Int(5,src2.d.itype));
+    var step1 := evalADD(OperandContents(lvm_s0,src2).itype.size,OperandContents(lvm_s0,src1),val.d);
+
+
+    ghost var lvm_b2, lvm_s2 := lvm_lemma_Add(lvm_b1, lvm_s0, lvm_sM, src2, size,src1,val,o);
+
+
+    assert OperandContents(lvm_s2, src2).val == step1.val;
+    assert OperandContents(lvm_s2,src2).val == evalADD(size,OperandContents(lvm_s0,src1),OperandContents(lvm_s0,val)).val;
+    assert OperandContents(lvm_s0, src1) == OperandContents(lvm_s2, src1); 
+
+    assert  lvm_require(lvm_b2, lvm_code_Add(dst, size,src2,val2), lvm_s2, lvm_sM,dst);
+    var step2 := evalADD(OperandContents(lvm_s2,dst).itype.size,OperandContents(lvm_s2,src2),val2.d);
+
+    ghost var lvm_b3, lvm_s3 := lvm_lemma_Add(lvm_b2, lvm_s2, lvm_sM, dst, size,src2,val2,o);
+    assert OperandContents(lvm_s3, dst).val 
+        == evalADD(OperandContents(lvm_s2,dst).itype.size,OperandContents(lvm_s2,src2),val2.d).val;
+  
+    assert OperandContents(lvm_s3, dst).val  == step2.val;
+
+    assert lvm_b3.hd.ins == RET(D(Void));
+
+    
+    ghost var lvm_b4, lvm_s4 := lvm_lemma_Ret(lvm_b3, lvm_s3, lvm_sM, dst, D(Void));
+    assert lvm_b4.CNil?;
+
+    lvm_sM := lvm_lemma_empty(lvm_s4,lvm_sM);
+    assert OperandContents(lvm_sM, dst).val  == step2.val;
+
+    assert evalCode_lax(lvm_cM, lvm_s0, lvm_sM,dst);
+    assert OperandContents(lvm_s0, src1) == OperandContents(lvm_sM, src1); 
+
+    assert OperandContents(lvm_sM, dst).val == step2.val;
+    assert  OperandContents(lvm_sM, dst).val == evalADD(OperandContents(lvm_s0,dst).itype.size,OperandContents(lvm_s0,src2),val2.d).val;
+    assert ValidState(lvm_sM);
+
+    reveal_evalCodeOpaque();
+}
 
 
 }
