src/Dafny/examples/challengeProblem1Simplified.i.dfy
@@ -58,7 +58,7 @@ lemma lvm_lemma_simple_challenge1(lvm_b0:lvm_codes, lvm_s0:lvm_state, lvm_sN:lvm
   reveal_lvm_RET();
   reveal_ValidData();
   reveal_evalCodeOpaque();
-  reveal_lvm_GetElementPtr();
+  reveal_lvm_code_GetElementPtr();
   reveal_eval_code();
 
   assert lvm_simple_challenge1(dst,t,op1,op2).Block?;
@@ -105,20 +105,6 @@ lemma lvm_lemma_simple_challenge1(lvm_b0:lvm_codes, lvm_s0:lvm_state, lvm_sN:lvm
   // assert exists r' :: evalCode(lvm_b0.hd, lvm_s0, r',dst);
   // assert lvm_b0.hd.Ins?;
   assert evalBlock(lvm_b0, lvm_s0, lvm_sN,dst);
-  // assert lvm_b0.hd.Block? && !lvm_b0.hd.block.CNil?;
-  // var r':state :| evalCode(lvm_b0.hd, lvm_s0, r',dst) && evalBlock(lvm_b0.tl, r', lvm_sN,dst);
-  // assert lvm_b0.hd.block.hd.Ins? && lvm_b0.hd.block.hd.ins == getelementins;
-
-  // assert evalCode(lvm_b0.hd, lvm_s0, r',dst);
-  // var evalBlock1:codes := lvm_b0.hd.block;
-  // assert evalBlock(evalBlock1,lvm_s0, r',dst);
-  // assert !evalBlock1.CNil?;
-  
-  // var r'':state :| evalCode(evalBlock1.hd, lvm_s0, r'',dst) && evalBlock(evalBlock1.tl, r'', r',dst); 
-  // assert evalIns(evalBlock1.hd.ins, lvm_s0, r'',dst);
-
-  // assert r''.ok;
-  // // assert r'.ok;
 
   ghost var lvm_ltmp1, lvm_cM:lvm_code, lvm_ltmp2 := lvm_lemma_block(lvm_b0, lvm_s0, lvm_sN,dst);
   lvm_sM := lvm_ltmp1;
@@ -154,7 +140,132 @@ lemma lvm_lemma_simple_challenge1(lvm_b0:lvm_codes, lvm_s0:lvm_state, lvm_sN:lvm
 }
 
 
+// ----*****-----
 
+
+function method{:opaque} lvm_simple_challenge1_cont(dst:lvm_operand_opr,s:MemState,t:bitWidth,op1:lvm_operand_opr,op2:lvm_operand_opr):lvm_code
+{
+    //getelementptr
+    reveal_IntFits();
+    var void := D(Void);
+    var ptrVar:lvm_operand_opr := D(Void);
+    var index := D(Int(2,IntType(8,false)));
+
+    lvm_Block(lvm_CCons(Ins(GETELEMENTPTR(dst,1,op1,index)),
+              lvm_CCons(Ins(LOAD(dst,s,1,dst)),
+              lvm_CCons(Ins(RET(void)),lvm_CNil()))))
+    // lvm_Block(lvm_CCons(Ins(GETELEMENTPTR(dst,t,op1,op2)),
+    //           lvm_CCons(Ins(RET(void)),lvm_CNil())))
+
+}
+
+lemma lvm_lemma_simple_challenge1_cont(lvm_b0:lvm_codes, lvm_s0:lvm_state, lvm_sN:lvm_state, 
+            dst:lvm_operand_opr,s:MemState,t:bitWidth,op1:lvm_operand_opr,op2:lvm_operand_opr)
+  returns (lvm_bM:lvm_codes, lvm_sM:lvm_state)
+  
+  requires lvm_require(lvm_b0, lvm_simple_challenge1_cont(dst,s,t,op1,op2), lvm_s0, lvm_sN,dst)
+  requires lvm_is_dst_opr(dst, lvm_s0)
+  requires lvm_is_src_opr(op1, lvm_s0)
+  requires lvm_get_ok(lvm_s0)
+
+  requires ValidOperand(lvm_s0,op1);
+  requires ValidOperand(lvm_s0,op2);
+  requires OperandContents(lvm_s0,op1).Ptr?;
+  requires OperandContents(lvm_s0,op1).bid in lvm_s0.m.mem; //needed for IsValidBid for valid input
+  requires ValidOperand(lvm_s0,dst)
+//   
+  ensures  lvm_ensure(lvm_b0, lvm_bM, lvm_s0, lvm_sM, lvm_sN,dst)
+  ensures  lvm_get_ok(lvm_sM)
+  ensures ValidOperand(lvm_sM,dst)
+
+  ensures OperandContents(lvm_sM,dst).Ptr?;
+  ensures  OperandContents(lvm_sM, dst) == evalGETELEMENTPTR(lvm_s0.m,1,OperandContents(lvm_s0,op1),Int(2,IntType(8,false)));
+  // ensures  lvm_state_eq(lvm_sM, lvm_update_ok(lvm_sM, lvm_update_mem( lvm_sM, lvm_s0)))
+{
+  reveal_lvm_simple_challenge1_cont();
+  reveal_lvm_RET();
+  reveal_ValidData();
+  reveal_evalCodeOpaque();
+  reveal_lvm_code_GetElementPtr();
+  reveal_eval_code();
+
+  assert lvm_simple_challenge1_cont(dst,s,t,op1,op2).Block?;
+  var getelementins := lvm_simple_challenge1_cont(dst,s,t,op1,op2).block.hd.ins;
+  assert lvm_simple_challenge1_cont(dst,s,t,op1,op2) == lvm_b0.hd;
+  // Check getelementins validity
+  assert getelementins.GETELEMENTPTR?;
+  assert ValidState(lvm_s0); 
+  assert MemValid(lvm_s0.m);
+  assert ValidOperand(lvm_s0,getelementins.dst);
+  assert ValidOperand(lvm_s0,getelementins.op1);
+  assert ValidOperand(lvm_s0,getelementins.op2);
+  assert OperandContents(lvm_s0,getelementins.op1).Ptr?;
+  assert OperandContents(lvm_s0,getelementins.op2).Int?;
+  assert !OperandContents(lvm_s0,getelementins.op2).itype.signed;
+  assert IsValidBid(lvm_s0.m,OperandContents(lvm_s0,getelementins.op1).bid);
+  // assert IsValidPtr(lvm_s0.m,OperandContents(lvm_s0,getelementins.op1).bid,OperandContents(lvm_s0,getelementins.op1).offset);
+  // assert OperandContents(lvm_s0,getelementins.op1).offset 
+      //  + (OperandContents(lvm_s0,getelementins.op2).val * getelementins.t)
+        //  < |lvm_s0.m.mem[OperandContents(lvm_s0,getelementins.op1).bid]|;
+  //
+  assert ValidInstruction(lvm_s0,getelementins);
+
+  var lvm_old_s:lvm_state := lvm_s0;
+  var two :=D(Void);
+      // var lvm_old_s:lvm_state := lvm_s0;
+  // assert evalCode(Ins(getelementins), lvm_s0, lvm_sN,dst);
+  assert lvm_s0.ok;
+  assert dst == getelementins.dst;
+  var getPtr := D(evalGETELEMENTPTR(lvm_s0.m,t,OperandContents(lvm_s0,getelementins.op1),OperandContents(lvm_s0,getelementins.op2)));
+  // assert getPtr.Ptr?;
+  // assert IsValidPtr(lvm_s0.m,getPtr.bid,getPtr.offset);
+  assert ValidData(lvm_sN,evalGETELEMENTPTR(lvm_s0.m,t,OperandContents(lvm_s0,getelementins.op1),OperandContents(lvm_s0,getelementins.op2)));
+  assert getPtr.D?;
+  assert getPtr.d == evalGETELEMENTPTR(lvm_s0.m,t,OperandContents(lvm_s0,getelementins.op1),OperandContents(lvm_s0,getelementins.op2));
+  // assert  lvm_sN == lvm_s0;
+  // assert evalUpdate(lvm_s0, getPtr, evalGETELEMENTPTR(lvm_s0.m,t,OperandContents(lvm_s0,getelementins.op1),OperandContents(lvm_s0,getelementins.op2)),lvm_sN);
+
+  // assert evalIns(getelementins,lvm_s0, lvm_sN,dst);
+  assert lvm_s0.ok;
+  // assert eval_code(lvm_Block(lvm_b0), lvm_s0, lvm_sN,dst);
+  // assert evalCode(lvm_Block(lvm_b0), lvm_s0, lvm_sN,dst);
+    assert !lvm_b0.CNil?;
+  // assert exists r' :: evalCode(lvm_b0.hd, lvm_s0, r',dst);
+  // assert lvm_b0.hd.Ins?;
+  assert evalBlock(lvm_b0, lvm_s0, lvm_sN,dst);
+
+  ghost var lvm_ltmp1, lvm_cM:lvm_code, lvm_ltmp2 := lvm_lemma_block(lvm_b0, lvm_s0, lvm_sN,dst);
+  lvm_sM := lvm_ltmp1;
+  lvm_bM := lvm_ltmp2;
+  var lvm_b1:lvm_codes := lvm_get_block(lvm_cM);
+  assert lvm_b1.lvm_CCons?;
+  assert lvm_b1.hd.Ins?;
+  assert lvm_b1.hd.ins.GETELEMENTPTR?;
+  // assert lvm_bM.lvm_CCons?;
+  assert lvm_b1.tl.lvm_CCons?;
+  assert lvm_b1.tl.hd.Ins?;
+  assert lvm_b1.tl.hd.ins.LOAD?;
+  assert lvm_b1.hd == Ins(GETELEMENTPTR(dst,1,op1,D(Int(2,IntType(8,false)))));
+
+  // ghost var lvm_ltmp3, lvm_b2, lvm_s2 := lvm_lemma_block(lvm_b1, lvm_s0, lvm_sM, dst);
+  ghost var lvm_b2, lvm_s2 := lvm_lemma_GetElementPtr(lvm_b1, lvm_s0, lvm_sM, dst, s,1,op1,D(Int(2,IntType(8,false))));
+  assert OperandContents(lvm_s2, dst) 
+        == evalGETELEMENTPTR(lvm_s0.m,1,OperandContents(lvm_s0,op1),Int(2,IntType(8,false)));
+  // assert lvm_sM.ok;
+  assert lvm_b2.hd.Ins?;
+  assert lvm_b2.hd.ins.LOAD?;
+  assert lvm_b2.hd.ins == LOAD(dst,s,1,dst);
+  
+  ghost var lvm_b3, lvm_s3 := lvm_lemma_Ret(lvm_b2, lvm_s2, lvm_sM, dst, D(Void));
+
+  lvm_sM := lvm_lemma_empty(lvm_s3,lvm_sM);
+
+  assert ValidState(lvm_sM);
+  // lvm_sM := lvm_lemma_empty(lvm_s2,lvm_sM);
+
+  assert evalCode_lax(lvm_cM, lvm_s0, lvm_sM,dst);
+  reveal_evalCodeOpaque();
+}
 
 
 }
