src/Dafny/examples/generalInstructions.i.dfy
@@ -6,7 +6,81 @@ module general_instructions {
     import opened control_flow
 
 
-function method{:opaque} lvm_GetElementPtr(dst:lvm_operand_opr,t:bitWidth,op1:lvm_operand_opr,op2:lvm_operand_opr):lvm_code
+function method{:opaque}lvm_code_Add(dst:lvm_operand_opr, size:nat, src1:lvm_operand_opr,src2:lvm_operand_opr):lvm_code
+
+{
+   Ins(ADD(dst, size,src1,src2))
+}
+lemma lvm_lemma_Add(lvm_b0:lvm_codes, lvm_s0:lvm_state, lvm_sN:lvm_state, 
+            dst:lvm_operand_opr, size:nat, src1:lvm_operand_opr,src2:lvm_operand_opr,o:operand)
+  returns (lvm_bM:lvm_codes, lvm_sM:lvm_state)
+
+  requires lvm_require(lvm_b0, lvm_code_Add(dst, size,src1,src2), lvm_s0, lvm_sN,dst)
+  requires lvm_is_dst_opr(dst, lvm_s0)
+  requires lvm_is_src_opr(src1, lvm_s0)
+  requires lvm_get_ok(lvm_s0)
+
+  requires ValidOperand(lvm_s0,src1);
+  requires OperandContents(lvm_s0,src1).Int?;
+  requires ValidOperand(lvm_s0,src2);
+  requires OperandContents(lvm_s0,src2).Int?;
+  requires ValidOperand(lvm_s0,dst);
+  requires OperandContents(lvm_s0,dst).Int?;
+
+  requires ValidOperand(lvm_s0,dst);
+  requires typesMatch(OperandContents(lvm_s0,src1),OperandContents(lvm_s0,src2))
+  requires OperandContents(lvm_s0,src2).Int?;
+  requires lvm_code_Add(dst, size,src1,src2).Ins?;
+  requires ValidOperand(lvm_s0,dst)
+// //   
+  ensures  lvm_ensure(lvm_b0, lvm_bM, lvm_s0, lvm_sM, lvm_sN,dst)
+  ensures  lvm_get_ok(lvm_sM)
+  ensures  ValidOperand(lvm_sM,dst)
+  ensures  ValidOperand(lvm_sM,src1)
+  ensures OperandContents(lvm_sM,src1).Int?;
+  ensures  ValidOperand(lvm_sM,src2)
+  ensures OperandContents(lvm_sM,src2).Int?;
+  ensures typesMatch(OperandContents(lvm_sM,src1),OperandContents(lvm_sM,src2))
+
+  ensures  OperandContents(lvm_sM,dst).Int?;
+  ensures  lvm_state_eq(lvm_sM, lvm_update_mem( lvm_sM, lvm_update_all(lvm_sM, lvm_s0)))
+  ensures  lvm_state_eq(lvm_sM, lvm_update_ok(lvm_sM, lvm_update_all( lvm_sM, lvm_s0)))
+  ensures  forall s2 :: evalCode(lvm_b0.hd, lvm_s0, s2,o) ==> s2.ok
+  ensures OperandContents(lvm_sM, dst).val == evalADD(OperandContents(lvm_s0,dst).itype.size,OperandContents(lvm_s0,src1),OperandContents(lvm_s0,src2)).val;
+  ensures ToTwosComp(OperandContents(lvm_sM, dst)).val == 
+          (OperandContents(lvm_s0, src1).val + OperandContents(lvm_s0, src2).val) % Pow256(OperandContents(lvm_s0, src1).itype.size)
+
+{
+    reveal_lvm_code_Add();
+    reveal_evalCodeOpaque();
+    reveal_eval_code();
+    assert lvm_code_Add(dst, size,src1,src2).Ins?;
+    var addIns := lvm_code_Add(dst, size,src1,src2).ins;
+    assert ValidInstruction(lvm_s0,addIns);
+
+    assert  ValidRegOperand(lvm_s0, dst);
+    assert ValidState(lvm_s0);
+    var lvm_old_s:lvm_state := lvm_s0;
+    assert evalCode_lax(lvm_Block(lvm_b0), lvm_s0, lvm_sN,dst);
+    assert lvm_s0.ok;
+    assert eval_code(lvm_Block(lvm_b0), lvm_s0, lvm_sN,dst);
+
+    ghost var lvm_ltmp1, lvm_cM:lvm_code, lvm_ltmp2 := lvm_lemma_block(lvm_b0, lvm_s0, lvm_sN,dst);
+    lvm_sM := lvm_ltmp1;
+    lvm_bM := lvm_ltmp2;
+    assert lvm_b0.tl == lvm_bM;
+    assert ValidState(lvm_s0);
+    assert lvm_s0.ok;
+    assert ValidState(lvm_sM);
+    assert ValidOperand(lvm_sM,dst);
+    assert evalIns(lvm_code_Add(dst, size,src1,src2).ins,lvm_s0,lvm_sM,dst);
+    assert evalUpdate(lvm_s0, dst, evalADD(OperandContents(lvm_s0,dst).itype.size,OperandContents(lvm_s0,src1),OperandContents(lvm_s0,src2)),lvm_sM);
+    assert ValidData(lvm_sM,evalADD(OperandContents(lvm_s0,dst).itype.size,OperandContents(lvm_s0,src1),OperandContents(lvm_s0,src2)));
+    assert OperandContents(lvm_sM, dst).val == evalADD(OperandContents(lvm_s0,dst).itype.size,OperandContents(lvm_s0,src1),OperandContents(lvm_s0,src2)).val;
+    reveal_evalCodeOpaque();
+}
+
+function method{:opaque} lvm_code_GetElementPtr(dst:lvm_operand_opr,t:bitWidth,op1:lvm_operand_opr,op2:lvm_operand_opr):lvm_code
 {
     //getelementptr
     reveal_IntFits();
@@ -18,7 +92,7 @@ lemma lvm_lemma_GetElementPtr(lvm_b0:lvm_codes, lvm_s0:lvm_state, lvm_sN:lvm_sta
             dst:lvm_operand_opr,s:MemState,t:bitWidth,op1:lvm_operand_opr,op2:lvm_operand_opr)
   returns (lvm_bM:lvm_codes, lvm_sM:lvm_state)
   
-  requires lvm_require(lvm_b0, lvm_GetElementPtr(dst,t,op1,op2), lvm_s0, lvm_sN,dst)
+  requires lvm_require(lvm_b0, lvm_code_GetElementPtr(dst,t,op1,op2), lvm_s0, lvm_sN,dst)
   requires lvm_is_dst_opr(dst, lvm_s0)
   requires lvm_is_src_opr(op1, lvm_s0)
   requires lvm_get_ok(lvm_s0)
@@ -40,7 +114,7 @@ lemma lvm_lemma_GetElementPtr(lvm_b0:lvm_codes, lvm_s0:lvm_state, lvm_sN:lvm_sta
   ensures  OperandContents(lvm_sM, dst) == evalGETELEMENTPTR(lvm_s0.m,t,OperandContents(lvm_s0,op1),OperandContents(lvm_s0,op2));
   ensures  lvm_state_eq(lvm_sM, lvm_update_ok(lvm_sM, lvm_update_all( lvm_sM, lvm_s0)))
 {
-  reveal_lvm_GetElementPtr();
+  reveal_lvm_code_GetElementPtr();
   reveal_ValidData();
   reveal_evalCodeOpaque();
   reveal_eval_code();
@@ -103,6 +177,76 @@ lemma lvm_lemma_Ret(lvm_b0:lvm_codes, lvm_s0:lvm_state, lvm_sN:lvm_state,dst:lvm
   reveal_evalCodeOpaque();
 }
 
+function method{:opaque} lvm_LOAD(dst:lvm_operand_opr,s:MemState,t:bitWidth,op1:lvm_operand_opr):lvm_code
+{
+    //getelementptr
+    reveal_IntFits();
+    Ins(LOAD(dst,s,t,op1))
 
+}
+
+
+
+lemma lvm_lemma_Load(lvm_b0:lvm_codes, lvm_s0:lvm_state, lvm_sN:lvm_state,dst:lvm_operand_opr,t:bitWidth,op1:lvm_operand_opr)
+  returns (lvm_bM:lvm_codes, lvm_sM:lvm_state)
+//   requires dst.LV?;
+  requires lvm_require(lvm_b0, lvm_LOAD(dst,lvm_s0.m,t,op1), lvm_s0, lvm_sN,dst)
+  requires lvm_is_dst_opr(dst, lvm_s0)
+  requires lvm_is_src_opr(op1, lvm_s0)
+  requires lvm_get_ok(lvm_s0)
+
+  requires ValidOperand(lvm_s0,op1);
+  requires ValidOperand(lvm_s0,dst);
+  requires OperandContents(lvm_s0,op1).Ptr?;
+  requires MemValid(lvm_s0.m);
+  requires IsValidPtr(lvm_s0.m,OperandContents(lvm_s0,op1).bid,OperandContents(lvm_s0,op1).offset);
+  requires lvm_s0 == lvm_sN; // this is the issue
+  requires exists d:Data :: Load(lvm_s0.m,lvm_sN.m,OperandContents(lvm_s0,op1).bid,OperandContents(lvm_s0,op1).offset,d);
+
+//   
+  ensures  lvm_ensure(lvm_b0, lvm_bM, lvm_s0, lvm_sM, lvm_sN,dst)
+  ensures  lvm_get_ok(lvm_sM)
+
+//   ensures  lvm_state_eq(lvm_sM,  lvm_s0)
+{
+  reveal_lvm_LOAD();
+  reveal_ValidData();
+  reveal_evalCodeOpaque();
+  reveal_eval_code();
+  reveal_ValidRegState();
+  reveal_ValidData();
+
+  assert evalBlock(lvm_b0, lvm_s0, lvm_sN,dst);
+  assert lvm_s0.ok;
+  assert ValidInstruction(lvm_s0,lvm_b0.hd.ins);
+
+  assert IsValidPtr(lvm_s0.m, OperandContents(lvm_s0,lvm_b0.hd.ins.src).bid,OperandContents(lvm_s0,lvm_b0.hd.ins.src).offset);
+  assert exists d:Data :: Load(lvm_s0.m,lvm_sN.m,OperandContents(lvm_s0,lvm_b0.hd.ins.src).bid,OperandContents(lvm_s0,lvm_b0.hd.ins.src).offset,d);
+  var d := evalLOAD(lvm_s0.m,lvm_sN.m,lvm_b0.hd.ins.t,OperandContents(lvm_s0,lvm_b0.hd.ins.src));
+  assert lvm_s0.m == lvm_sN.m;
+//   assert exists d:Data :: Load(lvm_s0.m,lvm_sN.m,OperandContents(lvm_s0,lvm_b0.hd.ins.src).bid,OperandContents(lvm_s0,lvm_b0.hd.ins.src).offset,d); 
+
+  assert lvm_s0.ok == lvm_sN.ok;
+  assert d == evalLOAD(lvm_s0.m,lvm_sN.m,lvm_b0.hd.ins.t,OperandContents(lvm_s0,lvm_b0.hd.ins.src));
+  assert D(d).D?;
+  assert evalUpdate(lvm_s0, D(d), evalLOAD(lvm_s0.m,lvm_sN.m,lvm_b0.hd.ins.t,OperandContents(lvm_s0,lvm_b0.hd.ins.src)),lvm_sN);
+
+  assert exists d:Data :: Load(lvm_s0.m,lvm_sN.m,OperandContents(lvm_s0,lvm_b0.hd.ins.src).bid,OperandContents(lvm_s0,lvm_b0.hd.ins.src).offset,d);
+//   assert dst.LV?;
+//   assert 
+//   assert evalLoad(lvm_s0,dst,OperandContents(lvm_s0,lvm_b0.hd.ins.src).bid,OperandContents(lvm_s0,lvm_b0.hd.ins.src).offset,lvm_sN);
+  
+//   assert evalIns(lvm_b0.hd.ins,lvm_s0,lvm_sN,dst);
+
+  ghost var lvm_ltmp1, lvm_cM:lvm_code, lvm_ltmp2 := lvm_lemma_block(lvm_b0, lvm_s0, lvm_sN,dst);
+  lvm_sM := lvm_ltmp1;
+  lvm_bM := lvm_ltmp2;
+
+  assert lvm_sM.ok;
+  assert lvm_b0.tl == lvm_bM;
+
+  assert ValidState(lvm_sM);
+  assert evalCode_lax(lvm_cM, lvm_s0, lvm_sM,dst);
+}
 
 }
